Added value trees

expression.v
@@ -2,6 +2,7 @@ Set Warnings "-notation-overridden,-parsing,-deprecated-hint-without-locality".
 From Coq Require Import Strings.String.
 Require Import PeanoNat.
 Require Import nvalue.
+Require Import value_tree.
 Require Import Bool.
 
 
@@ -9,21 +10,19 @@ Inductive ty : Type :=
   | Ty_Builtin : Type -> ty
   | Ty_Arrow : ty -> ty -> ty.
 
-Check Ty_Builtin nat.
-
-Inductive tm: Type :=
-  | tm_var : string -> tm
-  | tm_abs :string->string -> ty -> tm -> tm
-  | tm_app : tm -> tm -> tm
-  | tm_true : tm
-  | tm_false : tm
-  | tm_if0 : tm -> tm -> tm -> tm
-  | tm_const : nat -> tm
-  | tm_succ : tm -> tm
-  | tm_pred : tm -> tm 
-  | tm_mult : tm -> tm -> tm
-  | tm_nvalue (A:Type) : nvalue A -> tm
-  | tm_val : string -> tm -> tm -> tm.
+Inductive exp: Type :=
+  | exp_var : string -> exp
+  | exp_abs : string -> string -> ty -> exp -> exp
+  | exp_app : exp -> exp -> exp
+  | exp_val : string -> exp -> exp -> exp
+  | exp_if : exp -> exp -> exp -> exp
+  | exp_nvalue (A:Type) : nvalue A -> exp
+  | l_true : exp
+  | l_false : exp
+  | l_const : nat -> exp
+  | l_succ : exp -> exp
+  | l_pred : exp -> exp 
+  | l_mult : exp -> exp -> exp.
 
 Declare Custom Entry acnotation.
 
@@ -31,11 +30,11 @@ Declare Custom Entry acnotation.
 Notation "<{ e }>" := e (e custom acnotation at level 99).
 
 (*variable*)
-Coercion tm_var : string >-> tm.
+Coercion exp_var : string >-> exp.
 
 (*lambda*)
 Notation "'fun' name [ x :  t ]  { y }" :=
-  (tm_abs name x t y) (in custom acnotation at level 90, 
+  (exp_abs name x t y) (in custom acnotation at level 90, 
                      name at level 99,
                      x at level 99,
                      t custom acnotation at level 99,
@@ -44,11 +43,11 @@ Notation "'fun' name [ x :  t ]  { y }" :=
                      left associativity).
 
 (*application*)
-Notation "x y " := (tm_app x y) (in custom acnotation at level 1, left associativity).
+Notation "x y " := (exp_app x y) (in custom acnotation at level 1, left associativity).
 Notation "( x )" := x (in custom acnotation, x at level 99).
 Notation "x" := x (in custom acnotation at level 0, x constr at level 0).
 
-Notation "'val' name = x ; y" := (tm_val name x y) (in custom acnotation at level 90,
+Notation "'val' name = x ; y" := (exp_val name x y) (in custom acnotation at level 90,
                                                     name at level 99,
                                                     x custom acnotation at level 99,
                                                     y custom acnotation at level 99,
@@ -59,23 +58,23 @@ Notation "S -> T" := (Ty_Arrow S T) (in custom acnotation at level 50, right ass
 (*boolean*)
 Notation "'Bool'" := (Ty_Builtin bool) (in custom acnotation at level 0).
 Notation "'true'" := true (at level 1).
-Notation "'true'" := tm_true (in custom acnotation at level 0).
+Notation "'true'" := l_true (in custom acnotation at level 0).
 Notation "'false'" := false (at level 1).
-Notation "'false'" := tm_false (in custom acnotation at level 0).
+Notation "'false'" := l_false (in custom acnotation at level 0).
 
 (*natural numbers*)
 Notation "'Nat'" := (Ty_Builtin nat) (in custom acnotation at level 0).
-Notation "'succ' x" := (tm_succ x) (in custom acnotation at level 0,
+Notation "'succ' x" := (l_succ x) (in custom acnotation at level 0,
                                      x custom acnotation at level 0).
-Notation "'pred' x" := (tm_pred x) (in custom acnotation at level 0,
+Notation "'pred' x" := (l_pred x) (in custom acnotation at level 0,
                                      x custom acnotation at level 0).
-Notation "x * y" := (tm_mult x y) (in custom acnotation at level 1,
+Notation "x * y" := (l_mult x y) (in custom acnotation at level 1,
                                       left associativity).
-Coercion tm_const: nat >-> tm.
+Coercion l_const: nat >-> exp.
 
 (*if condition*)
-Notation "'if0' x 'then' y 'else' z" :=
-  (tm_if0 x y z) (in custom acnotation at level 89,
+Notation "'if' x 'then' y 'else' z" :=
+  (exp_if x y z) (in custom acnotation at level 89,
                     x custom acnotation at level 99,
                     y custom acnotation at level 99,
                     z custom acnotation at level 99,
@@ -87,54 +86,54 @@ Notation "[ x >> y ] m" := ( device _ x y m)(in custom acnotation at level 30,
                                             x at level 99, 
                                             y at level 99, 
                                             m custom acnotation at level 30).
-(* <{ [4 >> 6] [5 >> 9] [ > 6 ]}> *)
 
-Coercion tm_nvalue: nvalue >-> tm.
+Coercion exp_nvalue: nvalue >-> exp.
 Notation "'NvalueNat'" := (Ty_Builtin (nvalue nat)) (in custom acnotation at level 0).
 
 
-Inductive value : tm -> Prop :=
+Inductive value : exp -> Prop :=
   | v_abs : forall n x T2 t1,
       value <{fun n [x:T2] {t1}}>
   | v_true :
       value <{true}>
   | v_false :
       value <{false}>
-  | v_nat: forall (n:nat), value <{n}>.
+  | v_nat: forall (n:nat), value <{n}>
+  | v_nvalue: forall (A:Type) (n:nvalue A), value <{n}>.
 
 Reserved Notation "'/' x ':=' s '/' t" (in custom acnotation at level 20, x constr).
-Fixpoint subst (x : string) (s : tm) (t : tm) : tm :=
+Fixpoint subst (x : string) (s : exp) (t : exp) : exp :=
   match t with
-  | tm_var y =>
+  | exp_var y =>
       if String.eqb x y then s else t
   | <{fun n [y:T] {t1}}> =>
       if ((String.eqb x y) || (String.eqb x n)) then t else <{fun n [y:T] {/x:=s/ t1}}>
   | <{t1 t2}> =>
       <{(/x:=s/ t1) (/x:=s/ t2)}>
+  | <{val n = t1 ; t2}> =>
+      if (String.eqb x n) then t else <{val n = (/x:=s/ t1) ; (/x:=s/ t2)}>
+  | <{if t1 then t2 else t3}> =>
+        <{if (/x:=s/ t1) then (/x:=s/ t2) else (/x:=s/ t3)}>
+  | exp_nvalue x nv =>
+    <{nv}>
   | <{true}> =>
       <{true}>
   | <{false}> =>
       <{false}>
-  | <{if0 t1 then t2 else t3}> =>
-      <{if0 (/x:=s/ t1) then (/x:=s/ t2) else (/x:=s/ t3)}>
-  | tm_const n =>
+  | l_const n =>
     <{n}>
-  | tm_succ t1 =>
+  | l_succ t1 =>
     <{succ (/x:=s/ t1)}>
-  | tm_pred t1 =>
+  | l_pred t1 =>
     <{pred (/x:=s/ t1)}>
-  | tm_mult t1 t2 =>
+  | l_mult t1 t2 =>
     <{(/x:=s/ t1) * (/x:=s/ t2)}>
-  | tm_nvalue x nv =>
-    <{nv}>
-  | <{val n = t1 ; t2}> =>
-    if (String.eqb x n) then t else <{val n = (/x:=s/ t1) ; (/x:=s/ t2)}>
   end
 where "'/' x ':=' s '/' t" := (subst x s t) (in custom acnotation).
 Hint Constructors value : core.
 
 Reserved Notation "t '-->' t'" (at level 40). 
-Inductive step : tm -> tm -> Prop :=
+Inductive step : exp -> exp -> Prop :=
   | ST_AppAbs : forall n x T2 t1 v2,
          value v2 ->
          <{(fun n [x:T2] {t1}) v2}> --> <{ /n:=(fun n [x:T2] {t1})/ /x:=v2/ t1 }>
@@ -146,23 +145,19 @@ Inductive step : tm -> tm -> Prop :=
          t2 --> t2' ->
          <{v1 t2}> --> <{v1 t2'}>
   | ST_IfTrue : forall t1 t2,
-      <{if0 true then t1 else t2}> --> t1
+      <{if true then t1 else t2}> --> t1
   | ST_IfFalse : forall t1 t2,
-      <{if0 false then t1 else t2}> --> t2
+      <{if false then t1 else t2}> --> t2
   | ST_If : forall t1 t1' t2 t3,
       t1 --> t1' ->
-      <{if0 t1 then t2 else t3}> --> <{if0 t1' then t2 else t3}>
-
+      <{if t1 then t2 else t3}> --> <{if t1' then t2 else t3}>
   | ST_succ: forall (n:nat) (m:nat), m = S n -> <{succ n}> --> <{m}>
   | ST_succ_step: forall t t',  t --> t' -> <{succ t}> --> <{succ t'}>
-
   | ST_pred: forall (n:nat) (m:nat), m = Nat.pred n -> <{pred n}> --> <{m}>
   | ST_pred_step: forall t t',  t --> t' -> <{pred t}> --> <{pred t'}>
-
   | ST_prod: forall (n:nat) (m:nat) (r:nat), r = n * m -> <{n * m}> --> <{r}>
   | ST_prod_left: forall (n:nat) (n':nat) (m:nat), n --> n' -> <{n * m}> --> <{n' * m}>
   | ST_prod_right: forall (n:nat) (m:nat) (m':nat), m --> m' -> <{n * m}> --> <{n * m'}>
-
   | ST_Let1: forall n t1 t1' t2, t1 --> t1' -> 
             <{val n = t1 ; t2}> --> <{val n = t1' ; t2}>
   | ST_LetValue: forall n v1 t2, value v1 -> <{val n = v1 ; t2}> --> <{ /n:=v1/t2}>
@@ -182,52 +177,41 @@ Notation "t1 '-->*' t2" := (multistep t1 t2) (at level 40).
 
 
 Reserved Notation "t '==>' t'" (at level 40).
-Inductive bigstep : tm -> tm -> Prop :=
-
+Inductive bigstep : exp -> exp -> Prop :=
   | ST_Val : forall n t1 t2 w1 w2,
     <{t1}> ==> <{w1}> ->
     <{/n := w1/ t2 }> ==> <{w2}> ->
     <{val n = t1 ; t2}> ==> <{w2}>
-
   | ST_App : forall v t1 t2' t2 w,
     value v ->
     <{t1}> ==> v ->
     <{t2}> ==> <{t2'}> ->
     <{v t2'}> ==> <{w}> ->
     <{t1 t2}> ==> <{w}>
-
   | ST_Fun : forall n x T2 t1 v w,
     value v ->
     <{ /n:=(fun n [x:T2] {t1})/ /x:=v/ t1 }> ==> <{w}> ->
     <{(fun n [x:T2] {t1}) v}> ==> <{w}>
-
   | ST_Succ: forall (n:nat) w e, 
     w = S n ->
     <{e}> ==> <{n}> ->
     <{succ e}> ==> <{w}>
-
   | ST_Pred: forall (n:nat) w e, 
     w = Nat.pred n ->
     <{e}> ==> <{n}> ->
     <{pred e}> ==> <{w}>
-
   | ST_Prod: forall n (n':nat) m (m':nat) w, 
     w = n' * m' ->
     <{n}> ==> <{n'}> ->
     <{m}> ==> <{m'}> ->
     <{n * m}> ==> <{w}>
-
   | ST_If_T: forall t1 t2 t3,
     <{t1}> ==> <{true}> ->
-    <{if0 t1 then t2 else t3}> ==> <{t2}>
-
+    <{if t1 then t2 else t3}> ==> <{t2}>
   | ST_If_F: forall t1 t2 t3,
     <{t1}> ==> <{false}> ->
-    <{if0 t1 then t2 else t3}> ==> <{t3}>
-
+    <{if t1 then t2 else t3}> ==> <{t3}>
   | ST_Refl: forall t1, <{t1}> ==> <{t1}>
-
 where "t '==>' t'" := (bigstep t t').
-
 
 
