expression_test.v
@@ -1,6 +1,4 @@
 
-
-
 Require Import expression.
 Require Import String.
 Require Import Lia.
@@ -11,7 +9,7 @@ Definition x : string := "x".
 Definition y : string := "y".
 Definition z : string := "z".
 Definition n : string := "n".
-Definition fun0: string := "prod5". 
+Definition fun0: string := "fun0". 
 Definition prod5: string := "prod5". 
 
 Hint Unfold x : core.
@@ -19,7 +17,7 @@ Hint Unfold y : core.
 Hint Unfold z : core.
 
 Check <{x}>.
-Check <{fun prod5 [x:Nat] {x * 5} 5}>.
+Check <{fun prod5 [x:Nat] {x * [>5]} 5}>.
 Check <{x (fun prod5 [x:Nat] {x * 5})}>.
 Check <{val n = 25 ; n * 2}>.
 Check <{[4 >> 2][5 >> 5][6 >> 4][ > 5]}>.
@@ -33,15 +31,6 @@ Proof.
 intro n. eapply multi_step. apply ST_pred_step. apply ST_succ. auto.
 eapply multi_step. apply ST_pred. simpl. auto. apply multi_refl.
 Qed.
-
-(*Test of succ-pred*)
-Lemma smallstep_val:forall (n:nat),<{pred (succ n)}> -->* <{n}>.
-Proof.
-intros n0. induction n0 as [| n' Hd].
-- apply multi_step with (y := <{pred 1}>).
-  +apply ST_pred_step. apply ST_succ. reflexivity.
-  +apply multi_single. apply ST_pred. reflexivity.
-- rewrite Hd.
 
 (*Test of val*)
 Lemma smallstep_val: <{val n = (5*5) ; n * 2}> -->* 50.
@@ -64,28 +53,38 @@ Qed.
 
 (*BIG STEP SEMANTICS*)
 
-Lemma smallstep_pred_succ:forall (n:nat),<{pred (succ n)}> -->* <{n}>.
+(*Test of pred succ*)
+Lemma bigstep_pred_succ:forall (i:nat), <{pred (succ i)}> ==> <{i}>.
 Proof.
-intro n. eapply multi_step. apply ST_pred_step. apply ST_succ. auto.
-eapply multi_step. apply ST_pred. simpl. auto. apply multi_refl.
+intro i.
+apply ST_Pred with (n:=(S i)).
+-simpl. reflexivity.
+-apply ST_Succ with (n:=i). reflexivity. apply ST_Refl.
 Qed.
-
 
 (*Test of val*)
 Lemma bigstep_val: <{val n = (5*5) ; n * 2}> ==> 50.
 Proof.
 apply ST_Val with (w1:=25). 
--apply ST_Prod. reflexivity.
--simpl. apply ST_Prod. reflexivity.
+-apply ST_Prod with (n':=5)( m':=5). reflexivity. apply ST_Refl. apply ST_Refl.
+-simpl. apply ST_Prod with (n':=25)( m':=2). simpl. reflexivity. apply ST_Refl. apply ST_Refl.
 Qed.
 
+(*Test of fun*)
 Lemma bigstep_fun: <{fun prod5 [x:Nat] {x * 5} 5}> ==> 25.
 Proof.
 apply ST_Fun. simpl.
 - apply v_nat.
-- apply ST_Prod. reflexivity.
+- simpl. apply ST_Prod with (n':=5)(m':=5). reflexivity. apply ST_Refl. apply ST_Refl.
 Qed.
 
+(*Test of fun*)
+Lemma bigstep_nv_fun: <{fun prod5 [x:Nat] {x * [>5]} ([>5])}> ==> <{[>5]*[>5]}>.
+Proof.
+apply ST_Fun. simpl.
+- apply v_nvalue.
+- simpl. apply ST_Refl.
+Qed.
 
 
 
