value_tree.v
@@ -1,0 +1,40 @@
+Require Import String. 
+Require Import nvalue. 
+Require Import PeanoNat. 
+
+Inductive value_tree: Type :=
+| empty : list0 -> value_tree
+| some (B:Type) (A:nvalue B): list0  -> value_tree
+with list0 :=
+| nill : list0
+| cons : value_tree -> list0 -> list0.
+
+Definition extract_l (v:value_tree) : list0:= 
+match v with 
+| empty l => l
+| some _ _ l => l
+end.
+
+(*return empty value_tree if pos dowsn't exists*)
+Fixpoint pi (pos:nat) (v:value_tree): value_tree :=
+let ll := extract_l v in 
+match pos , ll with
+| (S n) ,(cons _ l) => pi n (empty l)
+| 0 , (cons vt _) => vt
+| (S n) , (nill) => empty nill
+| 0 , (nill) => empty nill
+end.
+
+
+
+
+
+
+
+
+
+
+
+
+
+
