value_tree_test.v
@@ -1,0 +1,23 @@
+
+Require Import String. 
+Require Import nvalue. 
+Require Import value_tree.
+Require Import Bool.
+
+Check (some nat (default nat 5) (cons (some bool (default bool true) nill) nill)).
+
+(*Returns first value tree in the list*)
+Compute (pi 0 (empty (cons (some bool (default bool true) nill) (cons (some bool (default bool false) nill) 
+(cons (some nat (default nat 5) nill) nill))))).
+
+(*Returns second value tree in the list*)
+Compute (pi 1 (empty (cons (some bool (default bool true) nill) (cons (some bool (default bool false) nill) 
+(cons (some nat (default nat 5) nill) nill))))).
+
+(*Returns third value tree in the list*)
+Compute (pi 2 (empty (cons (some bool (default bool true) nill) (cons (some bool (default bool false) nill) 
+(cons (some nat (default nat 5) nill) nill))))).
+
+(*Returns empty value tree*)
+Compute (pi 3 (empty (cons (some bool (default bool true) nill) (cons (some bool (default bool false) nill) 
+(cons (some nat (default nat 5) nill) nill))))).
